implementing eq for Seq and using it in mac, passing all F* universe regressions with haseq

src/ocaml-output/FStar_Parser_Dep.ml
@@ -322,7 +322,7 @@ with
 end))
 in (
 
-let ordered = ("fstar")::("prims")::("fstar.list.tot")::("fstar.functionalextensionality")::("fstar.predicateextensionality")::("fstar.set")::("fstar.heap")::("fstar.map")::("fstar.hyperheap")::("fstar.st")::("fstar.all")::[]
+let ordered = ("fstar")::("prims")::("fstar.list.tot")::("fstar.predicateextensionality")::("fstar.tset")::("fstar.functionalextensionality")::("fstar.set")::("fstar.heap")::("fstar.map")::("fstar.hyperheap")::("fstar.st")::("fstar.all")::[]
 in (
 
 let desired_opens = (FStar_Absyn_Const.fstar_ns_lid)::(FStar_Absyn_Const.prims_lid)::(FStar_Absyn_Const.st_lid)::(FStar_Absyn_Const.all_lid)::[]
