ulib/FStar.Heap.fst
@@ -1,6 +1,6 @@
 module FStar.Heap
 #set-options "--initial_fuel 0 --max_fuel 0 --initial_ifuel 1 --max_ifuel 1"
-open FStar.Set
+open FStar.TSet
 assume new type heap : Type0
 abstract type ref (a:Type) = 
   | MkRef of a //this implementation of ref is not realistic; it's just to get the universes right
@@ -38,39 +38,39 @@ assume SelConcat:     forall (a:Type) (h1:heap) (h2:heap) (a:ref a).       {:pat
                       if contains h2 a then sel (concat h1 h2) a==sel h2 a else sel (concat h1 h2) a==sel h1 a
 
 assume DomUpd:        forall (a:Type) (h:heap) (k1:ref a) (v:a).           {:pattern domain (upd h k1 v)}
-                      domain (upd h k1 v) == Set.union (domain h) (Set.singleton (Ref k1))
+                      domain (upd h k1 v) == union (domain h) (singleton (Ref k1))
 
 assume DomRestrict:   forall (h:heap) (r:set aref).                        {:pattern domain (restrict h r)}
-                      domain (restrict h r) == Set.intersect (domain h) r
+                      domain (restrict h r) == intersect (domain h) r
 
 assume DomConcat:     forall (h1:heap) (h2:heap).                          {:pattern domain (concat h1 h2)}
-                      domain (concat h1 h2)  == Set.union (domain h1) (domain h2)
+                      domain (concat h1 h2)  == union (domain h1) (domain h2)
 
-assume DomEmp:        domain emp == (Set.empty #aref)
+assume DomEmp:        domain emp == (empty #aref)
 
 assume DomContains:   forall (a:Type) (h:heap) (r:ref a).                  {:pattern contains h r}
-	              contains h r <==> Set.mem (Ref r) (domain h)
+	              contains h r <==> mem (Ref r) (domain h)
 
 type on (r:set aref) (p:(heap -> Type)) (h:heap) = p (restrict h r)
 type fresh (refs:set aref) (h0:heap) (h1:heap) =
   (forall (a:Type) (a:ref a).{:pattern (contains h0 a)} mem (Ref a) refs ==> not(contains h0 a) /\ contains h1 a)
 type modifies (mods:set aref) (h:heap) (h':heap) =
     equal h' (concat h' (restrict h (complement mods)))
-    /\ Set.subset (domain h) (domain h')
+    /\ subset (domain h) (domain h')
 
 abstract val lemma_modifies_trans: m1:heap -> m2:heap -> m3:heap
-                       -> s1:Set.set aref -> s2:Set.set aref
+                       -> s1:set aref -> s2:set aref
                        -> Lemma (requires (modifies s1 m1 m2 /\ modifies s2 m2 m3))
-                               (ensures (modifies (Set.union s1 s2) m1 m3))
+                               (ensures (modifies (union s1 s2) m1 m3))
 let lemma_modifies_trans m1 m2 m3 s1 s2 = ()
 
-let only x = Set.singleton (Ref x)
+let only x = singleton (Ref x)
 
 (* val op_Hat_Plus_Plus<u> : #a:Type(u) -> r:ref a -> set (aref<u>) -> Tot (set (aref<u>)) *)
-let op_Hat_Plus_Plus (#a:Type) r s = Set.union (Set.singleton (Ref r)) s
+let op_Hat_Plus_Plus (#a:Type) r s = union (singleton (Ref r)) s
 
 (* val op_Plus_Plus_Hat<u> : #a:Type(u) -> set (aref<u>) -> r:ref a -> Tot (set (aref<u>)) *)
-let op_Plus_Plus_Hat (#a:Type) s r = Set.union s (Set.singleton (Ref r))
+let op_Plus_Plus_Hat (#a:Type) s r = union s (singleton (Ref r))
 
 (* val op_Hat_Plus_Hat<u> : #a:Type(u) -> #b:Type(u) -> ref a -> ref b -> Tot (set (aref<u>)) *)
-let op_Hat_Plus_Hat (#a:Type) (#b:Type) r1 r2 = Set.union (Set.singleton (Ref r1)) (Set.singleton (Ref r2))
+let op_Hat_Plus_Hat (#a:Type) (#b:Type) r1 r2 = union (singleton (Ref r1)) (singleton (Ref r2))
