ulib/FStar.Set.fst
@@ -16,64 +16,64 @@
 *)
 module FStar.Set
 #set-options "--initial_fuel 0 --max_fuel 0 --initial_ifuel 0 --max_ifuel 0"
-open FStar.PredicateExtensionality
+open FStar.FunctionalExtensionality
 
-abstract type set a = a -> Tot Type0
-abstract type equal (#a:Type) (s1:set a) (s2:set a) = peq s1 s2
+abstract type set (a:eqtype) = a -> Tot bool
+abstract type equal (#a:eqtype) (s1:set a) (s2:set a) = feq s1 s2
 
 (* destructors *)
 
-abstract val mem : 'a -> set 'a -> Tot Type0
-let mem x s = s x
+abstract val mem : #a:eqtype -> a -> set a -> Tot bool
+let mem #a x s = s x
 
 (* constructors *)
-abstract val empty      : #a:Type -> Tot (set a)
-abstract val singleton  : 'a -> Tot (set 'a)
-abstract val union      : set 'a -> set 'a -> Tot (set 'a)
-abstract val intersect  : set 'a -> set 'a -> Tot (set 'a)
-abstract val complement : set 'a -> Tot (set 'a)
+abstract val empty      : #a:eqtype -> Tot (set a)
+abstract val singleton  : #a:eqtype -> a -> Tot (set a)
+abstract val union      : #a:eqtype -> set a -> set a -> Tot (set a)
+abstract val intersect  : #a:eqtype -> set a -> set a -> Tot (set a)
+abstract val complement : #a:eqtype -> set a -> Tot (set a)
 
-let empty           = fun #a x -> False
-let singleton x     = fun y -> y == x
-let union s1 s2     = fun x -> s1 x \/ s2 x
-let intersect s1 s2 = fun x -> s1 x /\ s2 x
-let complement s    = fun x -> ~ (s x)
+let empty              = fun #a x -> false
+let singleton #a x     = fun y -> y = x
+let union #a s1 s2     = fun x -> s1 x || s2 x
+let intersect #a s1 s2 = fun x -> s1 x && s2 x
+let complement #a s    = fun x -> not (s x)
 
 (* ops *)
-type subset (#a:Type) (s1:set a) (s2:set a) :Type0 = forall x. mem x s1 ==> mem x s2
+type subset (#a:eqtype) (s1:set a) (s2:set a) :Type0 = forall x. mem x s1 ==> mem x s2
 
 (* Properties *)
-abstract val mem_empty: #a:Type -> x:a -> Lemma
+abstract val mem_empty: #a:eqtype -> x:a -> Lemma
    (requires True)
-   (ensures (~ (mem x empty)))
+   (ensures (not (mem x empty)))
    [SMTPat (mem x empty)]
 
-abstract val mem_singleton: #a:Type -> x:a -> y:a -> Lemma
+abstract val mem_singleton: #a:eqtype -> x:a -> y:a -> Lemma
    (requires True)
-   (ensures (mem y (singleton x) <==> (x==y)))
+   (ensures (mem y (singleton x) = (x=y)))
    [SMTPat (mem y (singleton x))]
 
-abstract val mem_union: #a:Type -> x:a -> s1:set a -> s2:set a -> Lemma
+abstract val mem_union: #a:eqtype -> x:a -> s1:set a -> s2:set a -> Lemma
    (requires True)
-   (ensures (mem x (union s1 s2) == (mem x s1 \/ mem x s2)))
+   (ensures (mem x (union s1 s2) = (mem x s1 || mem x s2)))
    [SMTPat (mem x (union s1 s2))]
 
-abstract val mem_intersect: #a:Type -> x:a -> s1:set a -> s2:set a -> Lemma
+abstract val mem_intersect: #a:eqtype -> x:a -> s1:set a -> s2:set a -> Lemma
    (requires True)
-   (ensures (mem x (intersect s1 s2) == (mem x s1 /\ mem x s2)))
+   (ensures (mem x (intersect s1 s2) = (mem x s1 && mem x s2)))
    [SMTPat (mem x (intersect s1 s2))]
 
-abstract val mem_complement: #a:Type -> x:a -> s:set a -> Lemma
+abstract val mem_complement: #a:eqtype -> x:a -> s:set a -> Lemma
    (requires True)
-   (ensures (mem x (complement s) == ~(mem x s)))
+   (ensures (mem x (complement s) = not (mem x s)))
    [SMTPat (mem x (complement s))]
 
-abstract val mem_subset: #a:Type -> s1:set a -> s2:set a -> Lemma
+abstract val mem_subset: #a:eqtype -> s1:set a -> s2:set a -> Lemma
    (requires (forall x. mem x s1 ==> mem x s2))
    (ensures (subset s1 s2))
    [SMTPat (subset s1 s2)]
 
-abstract val subset_mem: #a:Type -> s1:set a -> s2:set a -> Lemma
+abstract val subset_mem: #a:eqtype -> s1:set a -> s2:set a -> Lemma
    (requires (subset s1 s2))
    (ensures (forall x. mem x s1 ==> mem x s2))
    [SMTPat (subset s1 s2)]
@@ -88,17 +88,17 @@ let mem_subset     #a s1 s2   = ()
 
 (* extensionality *)
 
-abstract val lemma_equal_intro: #a:Type -> s1:set a -> s2:set a -> Lemma
-    (requires  (forall x. mem x s1 <==> mem x s2))
+abstract val lemma_equal_intro: #a:eqtype -> s1:set a -> s2:set a -> Lemma
+    (requires  (forall x. mem x s1 = mem x s2))
     (ensures (equal s1 s2))
     [SMTPatT (equal s1 s2)]
 
-abstract val lemma_equal_elim: #a:Type -> s1:set a -> s2:set a -> Lemma
+abstract val lemma_equal_elim: #a:eqtype -> s1:set a -> s2:set a -> Lemma
     (requires (equal s1 s2))
     (ensures  (s1 == s2))
     [SMTPatT (equal s1 s2)]
 
-abstract val lemma_equal_refl: #a:Type -> s1:set a -> s2:set a -> Lemma
+abstract val lemma_equal_refl: #a:eqtype -> s1:set a -> s2:set a -> Lemma
     (requires (s1 == s2))
     (ensures  (equal s1 s2))
     [SMTPatT (equal s1 s2)]
@@ -106,3 +106,11 @@ abstract val lemma_equal_refl: #a:Type -> s1:set a -> s2:set a -> Lemma
 let lemma_equal_intro #a s1 s2 = ()
 let lemma_equal_elim  #a s1 s2 = ()
 let lemma_equal_refl  #a s1 s2 = ()
+
+(* TODO: how do we define these *)
+assume val set_to_tset: #key:eqtype -> set key -> Tot (TSet.set key)
+assume val lemma_set_to_tset:
+  #key:eqtype -> s:set key -> x:key
+  -> Lemma (requires (True))
+          (ensures (mem x s <==> TSet.mem x (set_to_tset s)))
+    [SMTPat (TSet.mem x (set_to_tset s))]
