examples/unit-tests/universes/testmref.fst
@@ -11,7 +11,7 @@ assume val z : ref int
 
 val test_frame_write_ref : unit -> ST unit
                               (requires (fun h -> y =!= z))
-                              (ensures (fun h0 x h1 -> modifies !{y} h0 h1))
+                              (ensures (fun h0 x h1 -> modifies (TSet.singleton (Ref y)) h0 h1))
 let test_frame_write_ref u =
   let v = !z in
   y := 17;
@@ -20,7 +20,7 @@ let test_frame_write_ref u =
 
 val test_frame_write_mref : unit -> ST unit
                               (requires (fun h -> y =!= MRef.as_ref x))
-                              (ensures (fun h0 x h1 -> modifies !{y} h0 h1))
+                              (ensures (fun h0 x h1 -> modifies (TSet.singleton (Ref y)) h0 h1))
 let test_frame_write_mref u =
   let v = MRef.read x in
   y := 17;
@@ -29,7 +29,7 @@ let test_frame_write_mref u =
 
 val test_frame_alloc_mref : unit -> ST unit
                               (requires (fun h -> MRef.contains h x))
-                              (ensures (fun h0 x h1 -> modifies !{y} h0 h1))
+                              (ensures (fun h0 x h1 -> modifies (TSet.singleton (Ref y)) h0 h1))
 let test_frame_alloc_mref u =
   let h0 = get() in
   assert (MRef.contains h0 x);
@@ -51,7 +51,7 @@ let test_frame_alloc_mref u =
 
 val test_write_mref : unit -> ST unit
                               (requires (fun h -> True))
-                              (ensures (fun h0 u h1 -> modifies !{MRef.as_ref x} h0 h1))
+                              (ensures (fun h0 u h1 -> modifies (TSet.singleton (Ref (MRef.as_ref x))) h0 h1))
 let test_write_mref u =
   let v = MRef.read x in
   MRef.write x (v + 1)
